RUXt/Model/Refute.lean
@@ -1,4 +1,4 @@
-import RUXt.Model.Summary
+import RUXt.Model.Witness
 
 namespace RUXt
 
@@ -8,16 +8,11 @@ namespace RUXt
 def DerivablePost (Λ : Library) (ςs : SummPicks) (f : Fid) (xs : List PVar)
     (τ : Ty) (ε : LExit) (Φ : Val → Tele.triple ςs -t> Asrt) : Prop :=
       -- Some function `f` outputs values of type `τ`
-      ∃ params body hdup, Λ.get f = some ⟨params, body, τ, hdup⟩ ∧
+      ∃ params body hdup, Λ.MapsTo f ⟨params, body, τ, hdup⟩ ∧
       -- The concrete input types must match the types in `ςs`
       xs = params.map Prod.fst ∧ ςs.map Prod.fst = params.map Prod.snd ∧
       -- `[ε : Φ]` is obtained from executing `f` after composing the summaries in `ςs`
-      ∃ L : Logic, L.DerivableSpec Λ
-        ⟨mergePosts ςs, (mergeVals ςs).map (fun vs => .call f (Term.ofVals vs)), ε, Φ⟩
-
-/-- Bind each summary in `ςs` to a variable in `xs` and calls `f` on `xs`. -/
-def Witness (f : Fid) (xs : List PVar) (ςs : SummPicks) : Tele.triple ςs -t> Expr :=
-  mergeSrcs xs ςs (.call f (Term.ofVars xs))
+      DerivableCall Λ f ςs ε Φ
 
 /-- The refutation procedure. -/
 def TryRefute (Λ : Library) (S : SummCtx) (r : SummCtx ⊕ Expr) : Prop :=
@@ -26,14 +21,14 @@ def TryRefute (Λ : Library) (S : SummCtx) (r : SummCtx ⊕ Expr) : Prop :=
   -- Construct [e : τ] that terminates with postcondition [ε : Φ]
   ∃ f xs τ ε Φ, DerivablePost Λ ςs f xs τ ε Φ ∧
   -- The postcondition is satisfiable
-  ∃ v args, sat ((Φ v).apply args) ∧
+  ∃ v args, Sat ((Φ v).apply args) ∧
   -- Case analysis on whether the derived state is Ok
   match r with
   | .inl S' => ε = .lok ∧ -- Case Ok: The summary context Σ is updated to Σ'
-        S' = SummCtx.update S τ ⟨Tele.triple ςs, Φ, Witness f xs ςs⟩
+        S' = SummCtx.update S τ ⟨Tele.triple ςs, Φ, witness f xs ςs⟩
   -- Found witness `e` for type unsoundness
   | .inr e => ε ≠ .lok ∧ --Cases Err/Miss: Found witness e for type unsoundness
-      e = (Witness f xs ςs).apply args
+      e = (witness f xs ςs).apply args
 
 /-- Meta-loop for deriving well-formed contexts. -/
 inductive WfSummCtx (Λ : Library) : SummCtx → Prop
@@ -46,28 +41,31 @@ inductive WfSummCtx (Λ : Library) : SummCtx → Prop
 /-! ### Inference soundness -/
 
 /-- Any derivable state can be witnessed by a main program. -/
-theorem DerivableForMain {Λ : Library} {S : SummCtx} {ςs : SummPicks} {f : Fid}
+theorem derivable_for_main {Λ : Library} {S : SummCtx} {ςs : SummPicks} {f : Fid}
     {xs : List PVar} {τ : Ty} {ε : LExit} {Q : Val → Tele.triple ςs -t> Asrt}
     (hsumm : ValidSummCtx Λ S) (hsub : S [⊐] ςs)
     (hpost : DerivablePost Λ ςs f xs τ ε Q) :
-    ReachableFromMain Λ τ (Witness f xs ςs) ε Q := by
-  sorry
+    ReachableFromMain Λ τ (witness f xs ςs) ε Q := by
+  obtain ⟨params, _, hdup, himpl, rfl, htypes, L, hspec⟩ := hpost
+  refine ⟨fun _ => witness_safeMain hsumm hsub himpl htypes, ?_⟩
+  refine witness_triple hsumm hsub hdup ?_ ⟨L, hspec⟩
+  simpa using congrArg List.length htypes.symm
 
 /-- Soundness of well-formed type summary contexts. -/
-theorem SummCtxSoundness {Λ : Library} {S : SummCtx}
+theorem summCtx_soundness {Λ : Library} {S : SummCtx}
     (hsumm : WfSummCtx Λ S) : ValidSummCtx Λ S := by
   induction hsumm with
   | nil =>
     intro τ ς hin
     rcases τ with ⟨kind⟩
-    · rw [baseSummCtxBase hin]
-      exact baseSummaryValid Λ kind
+    · rw [baseSummCtx_base hin]
+      exact baseSummary_valid Λ kind
     · contradiction
   | cons _ hrefute ih =>
     intro τ' ς' hin
     obtain ⟨ςs, hsub, f, xs, τ, ε, Φ, hpost, v, args, hsat, ⟨rfl, rfl⟩⟩ := hrefute
-    rcases SummCtx.memUpdate hin with ⟨rfl, rfl⟩ | hin
-    · exact ⟨DerivableForMain ih hsub hpost, v, args, hsat⟩
+    rcases SummCtx.mem_update hin with ⟨rfl, rfl⟩ | hin
+    · exact ⟨derivable_for_main ih hsub hpost, v, args, hsat⟩
     · exact ih τ' ς' hin
 
 /-! ### Soundness result of RUXt -/
@@ -77,24 +75,21 @@ def HasRefutedType (Λ : Library) (e : Expr) : Prop :=
   ∃ S, WfSummCtx Λ S ∧ TryRefute Λ S (.inr e)
 /-- A main program exhibits undefined behaviour. -/
 def Inadequate (Λ : Library) (e : Expr) : Prop :=
-  ∃ h, (Λ ⊢ ⟨∅ | e⟩ ⇓ ⟨h | .err⟩) ∧ ∃ τ, safeMain Λ e = some τ
+  ∃ h, (Λ ⊢ ⟨∅ | e⟩ ⇓ ⟨h | .err⟩) ∧ ∃ τ, SafeMain Λ e τ
 
 /-- Adequacy result for refuted type assignments. -/
 theorem inadequacy {Λ : Library} {e : Expr}
     (hrefuted : HasRefutedType Λ e) : Inadequate Λ e := by
   obtain ⟨S, hctx, hrefute⟩ := hrefuted
-  have hctx := SummCtxSoundness hctx
+  obtain hctx := summCtx_soundness hctx
   obtain ⟨ςs, hsub, f, xs, τ, εₗ, Φ, hpost, r, args, ⟨h', hΦ⟩, ⟨Hnok, rfl⟩⟩ := hrefute
-  obtain ⟨hsafe, hux⟩ := DerivableForMain hctx hsub hpost
-  obtain ⟨_, _, _, _, _, _, L, hspec⟩ := hpost
-  obtain hspec := L.ux_frame_soundness hspec
-  obtain ⟨_, _, ε, ⟨hε, _⟩⟩ := hspec _ _ _ hΦ
-  obtain ⟨h, hP, hstep⟩ := ux_frame_triple_spec hux _ _ _ hΦ _ hε
-  rw [teleBind_apply] at hP
-  rw [hP] at *
+  obtain ⟨hsafe, hux⟩ := derivable_for_main hctx hsub hpost
   refine ⟨h', ?_, τ, hsafe args⟩
-  rcases εₗ
-  · contradiction
+  obtain ⟨_, _, _, _, _, _, L, hspec⟩ := hpost
+  obtain ⟨_, _, ε, ⟨hε, _⟩⟩ := L.ux_frame_soundness hspec _ _ _ hΦ
+  obtain ⟨h, hP, hstep⟩ := ux_frame_triple_spec hux _ _ _ hΦ _ hε
+  rw [teleBind_apply] at hP; rw [hP] at *
+  rcases εₗ; contradiction
   · let .unit := r
     injection hε with hε; subst hε
     exact hstep
