RUXt/Model/Witness.lean
@@ -1,0 +1,122 @@
+import RUXt.Model.Summary
+
+namespace RUXt
+
+/-! ### Witness programs -/
+
+/-- Binds each summary in `ςs` to a variable in `xs` and calls `f` on `xs`. -/
+def witness (f : Fid) (xs : List PVar) (ςs : SummPicks) : Tele.triple ςs -t> Expr :=
+  mergeSrcs xs ςs (.call f (Term.ofVars xs))
+
+/-- A call to `f` on summaries `ςs` yields post `[ε:Φ]`. -/
+def DerivableCall (Λ : Library) (f : Fid) (ςs : SummPicks)
+    (ε : LExit) (Φ : Val → Tele.triple ςs -t> Asrt) : Prop :=
+  ∃ L : Logic, L.DerivableSpec Λ
+        ⟨mergePosts ςs, (mergeVals ςs).map (fun vs => .call f (Term.ofVals vs)), ε, Φ⟩
+
+/-! ### Type safety of witnesses -/
+
+private theorem mergeSrcs_safeProgram {Λ : Library} {ςs : SummPicks}
+    {𝕍 : VarCtx} {call : Expr} {τ : Ty} {args : TeleArg (Tele.triple ςs)}
+    {xs : List PVar} (Hlen : ςs.length = xs.length)
+    (hsafe : ∀ τ ς, (τ, ς) ∈ ςs → ∀ args, SafeMain Λ (ς.src.apply args) τ)
+    (hcall : SafeProgram (𝕍.consFrom xs (ςs.map Prod.fst)) Λ call τ) :
+    SafeProgram 𝕍 Λ ((mergeSrcs xs ςs call).apply args) τ := by
+  revert xs 𝕍
+  induction' ςs with ς ςs ih
+  · intro 𝕍 xs hlen hcall
+    obtain rfl := by simpa using hlen.symm
+    exact hcall
+  · intro 𝕍 xs hlen hcall
+    rcases xs with _ | ⟨x, xs⟩; contradiction
+    rcases args with ⟨v, rest⟩
+    rw [mergeSrcs_cons]; simp [SafeProgram]
+    refine ⟨ς.1, hsafe _ _ (by simp) _, ?_⟩
+    exact ih (by simp_all) (by simpa using hlen) hcall
+
+/-- Witness programs are safe main programs. -/
+theorem witness_safeMain {Λ : Library} {S : SummCtx} {ςs : SummPicks}
+    {args : TeleArg (Tele.triple ςs)} {f : Fid} {params : List (PVar × Ty)}
+    {body : Expr} {τ : Ty} {hdup : (params.map Prod.fst).Nodup}
+    (hsumm : ValidSummCtx Λ S) (hsub : S [⊐] ςs)
+    (himpl : Λ.MapsTo f ⟨params, body, τ, hdup⟩)
+    (htypes : ςs.map Prod.fst = params.map Prod.snd) :
+    SafeMain Λ ((witness f (params.map Prod.fst) ςs).apply args) τ := by
+  have hlen : ςs.length = (params.map Prod.fst).length := by
+    simpa using congrArg List.length htypes
+  obtain hsafe := fun τ ς h => (hsumm τ ς (hsub τ ς h)).1.1
+  refine mergeSrcs_safeProgram hlen hsafe ?_
+  rw [htypes, consVarCtx_eq_rev hdup]
+  exact safe_call himpl
+
+/-! ### Semantics of witnesses -/
+
+private theorem mergeSrcs_subst_nin {xs : List PVar} {ςs : SummPicks}
+    (hclosed : ∀ τ ς, (τ, ς) ∈ ςs → ∀ args, (ς.src.apply args).ClosedProgram)
+    {x : PVar} (hnin : x ∉ xs) {body : Expr} {v : Val} {args : TeleArg (Tele.triple ςs)}:
+    ((mergeSrcs xs ςs body).apply args).subst (.named x) v
+      = (mergeSrcs xs ςs (body.subst (.named x) v)).apply args := by
+  revert xs
+  induction' ςs with ς ςs ih
+  · simp
+  · intro xs hnin
+    rcases ς with ⟨τ, ς⟩
+    rcases args with ⟨_, rest⟩
+    simp [mergeSrcs_cons, Expr.subst, Expr.substTerm]
+    refine ⟨Expr.Closed.subst_eq (hclosed τ ς (by simp) _) _ (by tauto), ?_⟩
+    cases xs
+    · exact ih (fun τ ς h => hclosed τ ς (List.mem_cons_of_mem _ h)) (by tauto)
+    · simp at hnin; simp [if_neg (Ne.symm hnin.1)]
+      exact ih (fun τ ς h => hclosed τ ς (List.mem_cons_of_mem _ h)) hnin.2
+
+open scoped PFun
+
+private theorem witness_frame_step {Λ : Library} {ςs : SummPicks}
+    (hreach : ∀ τ ς, (τ, ς) ∈ ςs → ReachableFromMain Λ τ ς.src .lok ς.post)
+    {xs : List PVar} (hdup : xs.Nodup)
+    (hlen : xs.length = ςs.length)
+    {hF h h' : Heap} (hdisj : hF ##ₘ h)
+    {args : TeleArg (Tele.triple ςs)} (hpre: HProp h ((mergePosts ςs).apply args))
+    {body : Expr} {εₛ : Exit}
+    (hstep : Λ ⊢ ⟨hF ∪ h | body.substs xs (
+        Term.ofVals ((mergeVals ςs).apply args)
+    )⟩ ⇓ᵢ ⟨h' | εₛ⟩) :
+     Λ ⊢ ⟨hF | (mergeSrcs xs ςs body).apply args⟩ ⇓ᵢ ⟨h' | εₛ⟩ := by
+  revert body args xs hF h h'
+  induction' ςs with ς ςs ih
+  · simp_all
+  · intro xs hdup hlen hF h h' hdisjF args hpre body hstep
+    rcases xs with _ | ⟨x, xs⟩; contradiction
+    rcases args with ⟨v, rest⟩
+    rw [mergeSrcs_cons]
+    rw [mergePosts_cons] at hpre
+    obtain ⟨h1, h2, rfl, hdisj, hpre1, hpre2⟩ := hpre
+    obtain ⟨hdisjF1, hdisjF2⟩ := PFun.disjoint_union_r.1 hdisjF
+    rw [← PFun.union_assoc, mergeVals_cons] at hstep
+    obtain ⟨_, hux⟩ := hreach ς.1 ς.2 (by simp)
+    obtain ⟨h, hemp, εₛ, hε, hstep1⟩ := hux rest.fst v h1 hpre1
+    injection hε with hε; subst hε
+    simp [teleBind_apply] at hemp; subst hemp
+    rcases frame_addition hstep1 hF hdisjF1.symm with ⟨hstep1, _⟩ | ⟨l, Heq, _⟩
+    · simp_all; refine FrameStep.letIn hstep1 ?_
+      obtain hclosed := fun τ ς h args => safeMain_closed ((hreach τ ς (Or.inr h)).1 args)
+      rw [mergeSrcs_subst_nin hclosed hdup.1, PFun.union_comm hdisjF1.symm]
+      exact ih hdup.2 hlen (PFun.disjoint_union_l.2 ⟨hdisjF2, hdisj⟩) hpre2 hstep
+    · contradiction
+
+/-- Witness programs exhibit the same behaviour as a function call on the summaries. -/
+theorem witness_triple {Λ : Library} {S : SummCtx} {ςs : SummPicks}
+    {f : Fid} {xs : List PVar} {ε : LExit} {Φ : Val → Tele.triple ςs -t> Asrt}
+    (hsumm : ValidSummCtx Λ S) (hsub : S [⊐] ςs)
+    (hdup : xs.Nodup) (hlen : xs.length = ςs.length)
+    (hcall : DerivableCall Λ f ςs ε Φ) :
+    UXFrameTriple Λ (teleBind fun _ ↦ Asrt.emp, witness f xs ςs, ε, Φ) := by
+  intro args r h' hQ; rw [teleBind_apply]
+  obtain ⟨L, hspec⟩ := hcall
+  obtain ⟨h, hpre, εₛ, hε, hstep⟩ := L.ux_frame_soundness hspec args r h' hQ
+  rw [teleMap_apply] at hstep
+  refine ⟨∅, rfl, εₛ, hε, ?_⟩
+  obtain hreach := fun τ ς h => (hsumm τ ς (hsub τ ς h)).1
+  refine witness_frame_step hreach hdup hlen (PFun.disjoint_empty_l h) hpre ?_
+  rw [PFun.empty_union, Expr.substs_call (by rw [mergeVals_length]; exact hlen) hdup]
+  exact hstep
